@prefix dc: <http://purl.org/dc/elements/1.1/> .
@prefix dcat: <http://www.w3.org/ns/dcat#> .
@prefix dct: <http://purl.org/dc/terms/> .
@prefix euvoc: <http://publications.europa.eu/ontology/euvoc#> .
@prefix foaf: <http://xmlns.com/foaf/0.1/> .
@prefix mvreason: <https://radx.orgx/vocs/missing-value-reason/> .
@prefix org: <http://www.w3.org/ns/org#> .
@prefix owl: <http://www.w3.org/2002/07/owl#> .
@prefix pav: <http://purl.org/pav/> .
@prefix prov: <http://www.w3.org/ns/prov#> .
@prefix qb: <http://purl.org/linked-data/cube#> .
@prefix rdf: <http://www.w3.org/1999/02/22-rdf-syntax-ns#> .
@prefix rdfs: <http://www.w3.org/2000/01/rdf-schema#> .
@prefix schema: <http://schema.org/> .
@prefix sh: <http://www.w3.org/ns/shacl#> .
@prefix skos: <http://www.w3.org/2004/02/skos/core#> .
@prefix skosthes: <http://purl.org/iso25964/skos-thes#> .
@prefix skosxl: <http://www.w3.org/2008/05/skos-xl#> .
@prefix xsd: <http://www.w3.org/2001/XMLSchema#> .

<https://radx.orgx/vocs/missing-value-reason> a skos:ConceptScheme;
  dct:contributor <https://orcid.org/0000-0002-9381-9693>;
  dct:creator <https://orcid.org/0000-0001-6875-5360>;
  dct:description "List and document the reasons that can be used for missing values in the RADx systems."@en;
  dct:title "Missing value reasons in RADx"@en;
  pav:createdOn "2022-03-11T22:10:00-08:00"@en;
  pav:lastUpdatedOn "2022-03-23T15:01:00-08:00"@en;
  pav:version "0.0.5"@en;
  skos:hasTopConcept mvreason:MissingValue-9999;
  skos:prefLabel "Missing value reasons in RADx"@en .

mvreason:MissingValue-9999 a skos:Concept;
  skos:altLabel "0"@en;
  skos:definition "The value is missing"@en;
  skos:inScheme <https://radx.orgx/vocs/missing-value-reason>;
  skos:narrower mvreason:NotEnteredByOriginator-9960, mvreason:NotPresentedtoParticipant-9940,
    mvreason:NotSenttoDataHub-9980;
  skos:prefLabel "Missing Value (-9999)"@en;
  skos:topConceptOf <https://radx.orgx/vocs/missing-value-reason> .

mvreason:NotSenttoDataHub-9980 a skos:Concept;
  skos:altLabel "1"@en;
  skos:broader mvreason:MissingValue-9999;
  skos:definition "This information was not sent by the data aggregator (e.g., the Data Coordination Center) to the Data Hub"@en;
  skos:inScheme <https://radx.orgx/vocs/missing-value-reason>;
  skos:narrower mvreason:AnonymizationOrPrivacyConcerns-9986, mvreason:DataInvalid-9985,
    mvreason:DataLostOrInaccessible-9984, mvreason:DataTransferAgreement-9981, mvreason:NoParticipantConsenttoShare-9982,
    mvreason:NotAvailableOrMappable-9983, mvreason:OtherUnsentReasonNotSpecified-9987;
  skos:prefLabel "Not Sent to Data Hub (-9980)"@en .

mvreason:DataTransferAgreement-9981 a skos:Concept;
  skos:altLabel "1a"@en;
  skos:broader mvreason:NotSenttoDataHub-9980;
  skos:definition "Data originator's data transfer agreement with project precluded sending"@en;
  skos:inScheme <https://radx.orgx/vocs/missing-value-reason>;
  skos:prefLabel "Data Transfer Agreement (-9981)"@en .

mvreason:NoParticipantConsenttoShare-9982 a skos:Concept;
  skos:altLabel "1b"@en;
  skos:broader mvreason:NotSenttoDataHub-9980;
  skos:definition "Originator did not consent to its being provided"@en;
  skos:inScheme <https://radx.orgx/vocs/missing-value-reason>;
  skos:prefLabel "No Participant Consent to Share (-9982)"@en .

mvreason:NotAvailableOrMappable-9983 a skos:Concept;
  skos:altLabel "1c"@en;
  skos:broader mvreason:NotSenttoDataHub-9980;
  skos:definition "Reason from the originator was not available or mappable"@en;
  skos:inScheme <https://radx.orgx/vocs/missing-value-reason>;
  skos:prefLabel "Not Available Or Mappable (-9983)"@en .

mvreason:DataLostOrInaccessible-9984 a skos:Concept;
  skos:altLabel "1d"@en;
  skos:broader mvreason:NotSenttoDataHub-9980;
  skos:definition "Data was lost or inaccessible (unspecified reason)"@en;
  skos:inScheme <https://radx.orgx/vocs/missing-value-reason>;
  skos:prefLabel "Data Lost Or Inaccessible (-9984)"@en .

mvreason:DataInvalid-9985 a skos:Concept;
  skos:altLabel "1e"@en;
  skos:broader mvreason:NotSenttoDataHub-9980;
  skos:definition "Data was invalid (wrong format, wrong or unknown units, not parseable, or impossible value)"@en;
  skos:inScheme <https://radx.orgx/vocs/missing-value-reason>;
  skos:prefLabel "Data Invalid (-9985)"@en .

mvreason:AnonymizationOrPrivacyConcerns-9986 a skos:Concept;
  skos:altLabel "1f"@en;
  skos:broader mvreason:NotSenttoDataHub-9980;
  skos:definition "Data had anonymization/privacy concerns"@en;
  skos:inScheme <https://radx.orgx/vocs/missing-value-reason>;
  skos:prefLabel "Anonymization Or Privacy Concerns (-9986)"@en .

mvreason:OtherUnsentReasonNotSpecified-9987 a skos:Concept;
  skos:altLabel "1g"@en;
  skos:broader mvreason:NotSenttoDataHub-9980;
  skos:definition "Data was not sent to Data Hub for some reason not specified"@en;
  skos:inScheme <https://radx.orgx/vocs/missing-value-reason>;
  skos:prefLabel "Other Unsent Reason Not Specified (-9987)"@en .

mvreason:NotEnteredByOriginator-9960 a skos:Concept;
  dct:contributor <https://orcid.org/0000-0001-6875-5360>;
  skos:altLabel "2"@en;
  skos:broader mvreason:MissingValue-9999;
  skos:definition "This information was not provided by the originator (participant or sensor)"@en;
  skos:inScheme <https://radx.orgx/vocs/missing-value-reason>;
  skos:narrower mvreason:AllOriginatorsOmittedElement-9966, mvreason:CDEOmittedwithException-9967,
    mvreason:OmittedThisValue-9961, mvreason:OtherUnenteredReasonNotSpecified-9968, mvreason:RecordNotProvided-9965;
  skos:prefLabel "Not Entered By Originator (-9960)"@en .

mvreason:OmittedThisValue-9961 a skos:Concept;
  skos:altLabel "2a"@en;
  skos:broader mvreason:NotEnteredByOriginator-9960;
  skos:definition "Originator omitted this particular value. (If column, record, or CDE omitted *by the user*, choose that appropriate term here.)"@en;
  skos:inScheme <https://radx.orgx/vocs/missing-value-reason>;
  skos:narrower mvreason:AnswerNotKnown-9964, mvreason:OriginatorChosetoOmit-9962, mvreason:QuestionNotApplicable-9963;
  skos:prefLabel "Omitted This Value (-9961)"@en .

mvreason:OriginatorChosetoOmit-9962 a skos:Concept;
  skos:altLabel "2a.i"@en;
  skos:broader mvreason:OmittedThisValue-9961;
  skos:definition "Originator chose not to answer for personal reasons (unknown to data collector)"@en;
  skos:inScheme <https://radx.orgx/vocs/missing-value-reason>;
  skos:prefLabel "Originator Chose to Omit (-9962)"@en .

mvreason:QuestionNotApplicable-9963 a skos:Concept;
  skos:altLabel "2a.ii"@en;
  skos:broader mvreason:OmittedThisValue-9961;
  skos:definition "Originator deemed the question not applicable"@en;
  skos:inScheme <https://radx.orgx/vocs/missing-value-reason>;
  skos:prefLabel "Question Not Applicable (-9963)"@en .

mvreason:AnswerNotKnown-9964 a skos:Concept;
  skos:altLabel "2a.iii"@en;
  skos:broader mvreason:OmittedThisValue-9961;
  skos:definition "Originator did not know the answer"@en;
  skos:inScheme <https://radx.orgx/vocs/missing-value-reason>;
  skos:prefLabel "Answer Not Known (-9964)"@en .

mvreason:RecordNotProvided-9965 a skos:Concept;
  skos:altLabel "2b"@en;
  skos:broader mvreason:NotEnteredByOriginator-9960;
  skos:definition "Originator omitted this row (did not provide any answers for this record)"@en;
  skos:inScheme <https://radx.orgx/vocs/missing-value-reason>;
  skos:prefLabel "Record Not Provided (-9965)"@en .

mvreason:AllOriginatorsOmittedElement-9966 a skos:Concept;
  skos:altLabel "2c"@en;
  skos:broader mvreason:NotEnteredByOriginator-9960;
  skos:definition "Originator omitted this column/variable (this column/variable was not collected or could not be collected for any user"@en;
  skos:inScheme <https://radx.orgx/vocs/missing-value-reason>;
  skos:prefLabel "All Originators Omitted Element (-9966)"@en .

mvreason:CDEOmittedwithException-9967 a skos:Concept;
  skos:altLabel "2d"@en;
  skos:broader mvreason:NotEnteredByOriginator-9960;
  skos:definition "Originator omitted this CDE (category) due to NIH-approved exception"@en;
  skos:inScheme <https://radx.orgx/vocs/missing-value-reason>;
  skos:prefLabel "CDE Omitted with Exception (-9967)"@en .

mvreason:OtherUnenteredReasonNotSpecified-9968 a skos:Concept;
  skos:altLabel "2e"@en;
  skos:broader mvreason:NotEnteredByOriginator-9960;
  skos:definition "Originator did not provide data for some other reason"@en;
  skos:inScheme <https://radx.orgx/vocs/missing-value-reason>;
  skos:prefLabel "Other Unentered Reason Not Specified (-9968)"@en .

mvreason:NotPresentedtoParticipant-9940 a skos:Concept;
  dct:contributor <https://orcid.org/0000-0001-6875-5360>;
  skos:altLabel "3"@en;
  skos:broader mvreason:MissingValue-9999;
  skos:definition "This question (element) was not presented to the participant"@en;
  skos:inScheme <https://radx.orgx/vocs/missing-value-reason>;
  skos:narrower mvreason:CDENotPresentedDuetoException-9943, mvreason:ElementNeverPresentedforCollection-9944,
    mvreason:NoParticipantConsenttoAsk-9942, mvreason:OtherUnpresentedReasonNotSpecified-9946,
    mvreason:ProcessError-9945, mvreason:SkipLogic-9941;
  skos:prefLabel "Not Presented to Participant (-9940)"@en .

mvreason:SkipLogic-9941 a skos:Concept;
  skos:altLabel "3a"@en;
  skos:broader mvreason:NotPresentedtoParticipant-9940;
  skos:definition "Skip logic in the form or directions caused the question to not be presented"@en;
  skos:inScheme <https://radx.orgx/vocs/missing-value-reason>;
  skos:prefLabel "Skip Logic (-9941)"@en .

mvreason:NoParticipantConsenttoAsk-9942 a skos:Concept;
  skos:altLabel "3b"@en;
  skos:broader mvreason:NotPresentedtoParticipant-9940;
  skos:definition "Originator did not provide consent for question to be asked"@en;
  skos:inScheme <https://radx.orgx/vocs/missing-value-reason>;
  skos:prefLabel "No Participant Consent to Ask (-9942)"@en .

mvreason:CDENotPresentedDuetoException-9943 a skos:Concept;
  skos:altLabel "3c"@en;
  skos:broader mvreason:NotPresentedtoParticipant-9940;
  skos:definition "The CDE (or element of the CDE) was not presented due to CDE exception"@en;
  skos:inScheme <https://radx.orgx/vocs/missing-value-reason>;
  skos:prefLabel "CDE Not Presented Due to Exception (-9943)"@en .

mvreason:ElementNeverPresentedforCollection-9944 a skos:Concept;
  skos:altLabel "3d"@en;
  skos:broader mvreason:NotPresentedtoParticipant-9940;
  skos:definition "This element (question or variable) was not presented to user for collection (reason unspecified)"@en;
  skos:inScheme <https://radx.orgx/vocs/missing-value-reason>;
  skos:prefLabel "Element Never Presented for Collection (-9944)"@en .

mvreason:ProcessError-9945 a skos:Concept;
  skos:altLabel "3e"@en;
  skos:broader mvreason:NotPresentedtoParticipant-9940;
  skos:definition "A processing error caused the question to not be presented"@en;
  skos:inScheme <https://radx.orgx/vocs/missing-value-reason>;
  skos:prefLabel "Process Error (-9945)"@en .

mvreason:OtherUnpresentedReasonNotSpecified-9946 a skos:Concept;
  skos:altLabel "3f"@en;
  skos:broader mvreason:NotPresentedtoParticipant-9940;
  skos:definition "Question was not presented for some reason not specified"@en;
  skos:inScheme <https://radx.orgx/vocs/missing-value-reason>;
  skos:prefLabel "Other Unpresented Reason Not Specified (-9946)"@en .
